change abstract class blood and blood list to match python

verification/BloodList.dfy
@@ -1,101 +1,89 @@
 include "Blood.dfy"
 
-class {:autocontracts} BloodList
+class BloodList
 {
-  var list: array<Blood>;
-  var upto: int;
+    var list: array<Blood>;
+    var upto: int;
 
-  predicate Valid()
-  reads this;
-  {
-    list != null && 0 <= upto < list.Length
-  }
-
-  constructor(size: int)
-  requires size > 0;
-  ensures fresh(list);  
-  {
-    list := new Blood[size];
-    upto := 0;
-  }
-
-  method addBlood(blood: Blood)
-  ensures list[upto] == blood;
-  ensures upto == old(upto) + 1;
-  ensures old(list[0..old(upto)]) == list[0..old(upto)];
-  {
-   
-    if upto == list.Length - 1
+    predicate Valid()
+    reads this, this.list, this`upto;
     {
-      var newlist := new Blood[2*list.Length];
-      forall(i | 0 <= i < list.Length)
-      { 
-        newlist[i] := list[i];
-      }
-      list := newlist;
-    }
-    list[upto+1], upto := blood, upto + 1;
-
-
-  }
-
-
-  method removeBlood(blood: Blood)
-  requires upto > 0;
-  requires exists t :: 0 <= t <= upto && list[t] == blood;
-  ensures upto == old(upto) - 1;
-  ensures exists t :: 0 <= t <= old(upto) && old(list[t]) == blood
-                      && forall p :: 0 <= p < t ==> list[p] == old(list[p])
-                      && forall q :: t < q <= old(upto) ==> list[q-1] == old(list[q]);
-  {
-    var i:=0;
-    var bloodFound := false;
-    var bloodIndex := -1;
-    while i <= upto
-    invariant 0 <= i <= upto;
-    invariant forall k :: 0 <= k < i ==> list[k] != blood;
-    invariant forall j :: 0 <= j < i ==> list[j] == old(list[j])
-    invariant bloodFound ==> forall l :: bloodIndex < l < i ==> list[l-1] == old(list[l])
-    decreases upto - i;
-    {
-      if list[i] == blood
-      {
-          bloodFound := true;
-          bloodIndex := i;
-          forall(j | i < j <= upto)
-          {
-            list[j - 1] := list[j];
-          }
-
-          break;
-      }
-      i := i + 1;
+        list != null && list.Length > 0 && 0 <= upto <= list.Length
+        && forall i :: 0 <= i < upto ==> list[i] != null
     }
 
-    upto := upto - 1;
+    constructor(size: int)
+    requires size > 0;
+    ensures Valid(); 
+    ensures fresh(list);
+    modifies this, this.list, this`upto
+    {
+        list := new Blood[size];
+        upto := 0;
+    }
 
-  }
+
+    method addBlood(blood: Blood)
+    ensures Valid(); requires Valid();
+    requires blood != null
+    ensures upto > 0
+    ensures list[upto-1] == blood;
+    ensures upto == old(upto) + 1;
+    ensures old(upto) == old(list.Length) ==> fresh(list) && list.Length == 2*old(list).Length;
+    modifies this, this.list, this`upto
+    {
+        assert list.Length != 0;
+        if upto == list.Length
+        {
+            var newlist := new Blood[2*list.Length];
+            forall(i | 0 <= i < list.Length)
+            {
+                newlist[i] := list[i];
+            }
+            list := newlist;
+            assert upto < list.Length;
+        }
+        assert upto < list.Length;
+        list[upto], upto := blood, upto + 1;
+
+    }
+
+    
+    method extractBlood(id: int) returns (bloodFound: bool, blood: Blood)
+    ensures Valid(); requires Valid();
+    requires upto > 0;
+    ensures bloodFound ==> upto == old(upto) - 1;
+    ensures bloodFound ==> exists t :: 0 <= t < old(upto) && old(list[t]) == blood
+                        && forall p :: 0 <= p < t ==> list[p] == old(list[p])
+                        && forall q :: t < q < old(upto) ==> list[q-1] == old(list[q]);
+    ensures bloodFound ==> blood.id == id;
+    modifies this.list, this`upto;
+    {
+        bloodFound := false;
+        blood := null;
+        var i:=0;
+        var bloodIndex := -1;
+        while i < upto
+        invariant 0 <= i <= upto;
+        invariant forall k :: 0 <= k < i ==> list[k] != blood;
+        invariant forall j :: 0 <= j < i ==> list[j] == old(list[j])
+        invariant bloodFound ==> forall l :: bloodIndex < l < i ==> list[l-1] == old(list[l])
+        decreases upto - i;
+        {
+            if list[i].id == id
+            {
+                bloodFound := true;
+                bloodIndex := i;
+                blood := list[i];
+                forall(j | i < j < upto)
+                {
+                    list[j - 1] := list[j];
+                }
+                upto := upto - 1;
+                break;
+            }
+            i := i + 1;
+        }
+
+    }
 }
-
-
-/*
-method Main() {
-  var s:seq<int> := [20,18,33,44];
-  print s[..];
-  print "\n";
-  var m:seq<int> := RemoveBlood(s,44);
- // assert |m| == 3;
- // assert m[0] == 20;
-  //assert m[1] == 18;
-  //assert m[2] == 33;
- // assert 44 !in m;
-  print "After delete: ";
-  print m;
-  print "\n";
-  
-  var n:seq<int> := RemoveBlood(s,50);
-  print "After delete: ";
-  print n;
-  print "\n";
-  assert n==s;
-}*/
